lean-tracing-demo-ccfraft/Sparse.lean
@@ -32,6 +32,7 @@ import Sparse.NativeArrayQueue
 import Sparse.NativeArrayVote
 import Sparse.NativeEncodeProofs
 import Sparse.NativeInitialEncoding
+import Sparse.NativeObservationEncoding
 import Sparse.NativeNodeEncoding
 import Sparse.NativeQuorumEncoding
 import Sparse.NativeConstructors
